{
 "cells": [
  {
   "cell_type": "markdown",
   "metadata": {},
   "source": [
    "### Activity 2: Poisson distribution - mean and variance"
   ]
  },
  {
   "cell_type": "markdown",
   "metadata": {},
   "source": [
    "#### Consider a Poisson process with a rate parameter $\\lambda$. The probability of observing k events in a fixed interval is given by the Poisson distribution. \n",
    "\n",
    "##### 1. Write down the Poisson probability mass function $p(k \\mid \\lambda)$."
   ]
  },
  {
   "cell_type": "markdown",
   "metadata": {},
   "source": [
    "The probability mass function for observing \\( k \\) events in a fixed interval is\n",
    "\n",
    "$$\n",
    "p(k \\mid \\lambda) = \\frac{\\lambda^k e^{-\\lambda}}{k!},\n",
    "$$\n",
    "\n",
    "where \\( k = 0, 1, 2,... \\).\n"
   ]
  },
  {
   "cell_type": "markdown",
   "metadata": {},
   "source": [
    "##### 2. Compute the expectation value $<k>$."
   ]
  },
  {
   "cell_type": "markdown",
   "metadata": {},
   "source": [
    "The expectation value of \\( k \\) for a Poisson distribution is defined as\n",
    "\n",
    "$$\n",
    "\\langle k \\rangle = \\sum_{k=0}^{\\infty} k \\, p(k \\mid \\lambda).\n",
    "$$\n",
    "\n",
    "Plugging in the probability mass function $ p(k \\mid \\lambda) $:\n",
    "\n",
    "$$\n",
    "\\langle k \\rangle\n",
    "= \\sum_{k=0}^{\\infty} k \\frac{\\lambda^k e^{-\\lambda}}{k!}.\n",
    "$$\n",
    "\n",
    "The $ k = 0 $ term vanishes:\n",
    "\n",
    "$$\n",
    "\\langle k \\rangle\n",
    "= \\sum_{k=1}^{\\infty} k \\frac{\\lambda^k e^{-\\lambda}}{k!}.\n",
    "$$\n",
    "\n",
    "Using the identity\n",
    "\n",
    "$$\n",
    "\\frac{k}{k!} = \\frac{1}{(k-1)!},\n",
    "$$\n",
    "\n",
    "we obtain:\n",
    "\n",
    "$$\n",
    "\\langle k \\rangle\n",
    "= e^{-\\lambda} \\sum_{k=1}^{\\infty} \\frac{\\lambda^k}{(k-1)!}.\n",
    "$$\n",
    "\n",
    "Factoring out a power of $ \\lambda $:\n",
    "\n",
    "$$\n",
    "\\langle k \\rangle\n",
    "= \\lambda e^{-\\lambda} \\sum_{k=1}^{\\infty} \\frac{\\lambda^{k-1}}{(k-1)!}.\n",
    "$$\n",
    "\n",
    "Letting $ j = k - 1 $, this becomes:\n",
    "\n",
    "$$\n",
    "\\langle k \\rangle\n",
    "= \\lambda e^{-\\lambda} \\sum_{j=0}^{\\infty} \\frac{\\lambda^j}{j!}.\n",
    "$$\n",
    "\n",
    "Using the Taylor series expansion of the exponential function:\n",
    "\n",
    "$$\n",
    "\\sum_{j=0}^{\\infty} \\frac{\\lambda^j}{j!} = e^{\\lambda},\n",
    "$$\n",
    "\n",
    "we are left with:\n",
    "\n",
    "$$\n",
    "\\langle k \\rangle = \\lambda e^{-\\lambda} e^{\\lambda} = \\lambda.\n",
    "$$\n",
    "\n",
    "Therefore,\n",
    "\n",
    "$$\n",
    "\\boxed{\\langle k \\rangle = \\lambda.}\n",
    "$$\n"
   ]
  },
  {
   "cell_type": "markdown",
   "metadata": {},
   "source": [
    "##### 3. Compute the variance $\\mathrm{Var}(k)$."
   ]
  },
  {
   "cell_type": "markdown",
   "metadata": {},
   "source": [
    "The variance of k is given by **Bishop Eq. 1.51**:\n",
    "\n",
    "$$\n",
    "\\mathrm{Var}(k) = \\langle k^2 \\rangle - \\langle k \\rangle^2.\n",
    "$$\n",
    "\n",
    "For a Poisson distribution with parameter $ \\lambda $, we just calculated the expectation value to be:\n",
    "\n",
    "$$\n",
    "\\langle k \\rangle = \\lambda.\n",
    "$$\n",
    "\n",
    "Now computing $ \\langle k^2 \\rangle $:\n",
    "\n",
    "$$\n",
    "\\langle k^2 \\rangle\n",
    "= \\sum_{k=0}^{\\infty} k^2 \\, p(k \\mid \\lambda)\n",
    "= \\sum_{k=0}^{\\infty} k^2 \\frac{\\lambda^k e^{-\\lambda}}{k!}.\n",
    "$$\n",
    "\n",
    "Rewriting  $ \\langle k^2 \\rangle $ as $k^2 = k(k-1) + k$:\n",
    "\n",
    "$$\n",
    "\\langle k^2 \\rangle\n",
    "= \\sum_{k=0}^{\\infty} k(k-1)\\frac{\\lambda^k e^{-\\lambda}}{k!}\n",
    "+ \\sum_{k=0}^{\\infty} k\\frac{\\lambda^k e^{-\\lambda}}{k!}.\n",
    "$$\n",
    "\n",
    "The second sum is simply\n",
    "\n",
    "$$\n",
    "\\langle k \\rangle = \\lambda.\n",
    "$$\n",
    "\n",
    "For the first sum, note that $ \\frac{k(k-1)}{k!} = \\frac{1}{(k-2)!}$ and the terms with \\( k=0,1 \\) vanish. Thus:\n",
    "\n",
    "$$\n",
    "\\sum_{k=0}^{\\infty} k(k-1)\\frac{\\lambda^k e^{-\\lambda}}{k!}\n",
    "= e^{-\\lambda} \\sum_{k=2}^{\\infty} \\frac{\\lambda^k}{(k-2)!}.\n",
    "$$\n",
    "\n",
    "Factor out $ \\lambda^2 $:\n",
    "\n",
    "$$\n",
    "= \\lambda^2 e^{-\\lambda} \\sum_{k=2}^{\\infty} \\frac{\\lambda^{k-2}}{(k-2)!}.\n",
    "$$\n",
    "\n",
    "Letting $ j = k - 2 $, this becomes:\n",
    "\n",
    "$$\n",
    "= \\lambda^2 e^{-\\lambda} \\sum_{j=0}^{\\infty} \\frac{\\lambda^j}{j!}\n",
    "= \\lambda^2.\n",
    "$$\n",
    "\n",
    "Therefore,\n",
    "\n",
    "$$\n",
    "\\langle k^2 \\rangle = \\lambda^2 + \\lambda.\n",
    "$$\n",
    "\n",
    "Substituting into the variance:\n",
    "\n",
    "$$\n",
    "\\mathrm{Var}(k)\n",
    "= \\langle k^2 \\rangle - \\langle k \\rangle^2\n",
    "= (\\lambda^2 + \\lambda) - \\lambda^2\n",
    "= \\lambda.\n",
    "$$\n",
    "\n",
    "Therefore,\n",
    "\n",
    "$$\n",
    "\\boxed{\\mathrm{Var}(k) = \\langle k \\rangle.}\n",
    "$$\n"
   ]
  },
  {
   "cell_type": "markdown",
   "metadata": {},
   "source": [
    "##### 4. Show explicitly that $\\mathrm{Var}(k)$ = $\\langle k \\rangle$."
   ]
  },
  {
   "cell_type": "markdown",
   "metadata": {},
   "source": [
    "Start with the Poisson pmf:\n",
    "\n",
    "$$\n",
    "p(k\\mid \\lambda)=\\frac{\\lambda^k e^{-\\lambda}}{k!}, \\qquad k=0,1,2,\\dots\n",
    "$$\n",
    "\n",
    "The expectation value is\n",
    "\n",
    "$$\n",
    "\\langle k\\rangle=\\sum_{k=0}^{\\infty} k\\,p(k\\mid\\lambda)\n",
    "= e^{-\\lambda}\\sum_{k=1}^{\\infty} k\\frac{\\lambda^k}{k!}\n",
    "= e^{-\\lambda}\\sum_{k=1}^{\\infty}\\frac{\\lambda^k}{(k-1)!}.\n",
    "$$\n",
    "\n",
    "Factor out one power of $\\lambda$ and shift the index \\(j=k-1\\):\n",
    "\n",
    "$$\n",
    "\\langle k\\rangle\n",
    "= \\lambda e^{-\\lambda}\\sum_{k=1}^{\\infty}\\frac{\\lambda^{k-1}}{(k-1)!}\n",
    "= \\lambda e^{-\\lambda}\\sum_{j=0}^{\\infty}\\frac{\\lambda^j}{j!}\n",
    "= \\lambda.\n",
    "$$\n",
    "\n",
    "Now compute $\\langle k(k-1)\\rangle$:\n",
    "\n",
    "$$\n",
    "\\langle k(k-1)\\rangle\n",
    "= \\sum_{k=0}^{\\infty} k(k-1)p(k\\mid\\lambda)\n",
    "= e^{-\\lambda}\\sum_{k=2}^{\\infty} k(k-1)\\frac{\\lambda^k}{k!}.\n",
    "$$\n",
    "\n",
    "Use the identity\n",
    "\n",
    "$$\n",
    "\\frac{k(k-1)}{k!}=\\frac{1}{(k-2)!},\n",
    "$$\n",
    "\n",
    "so\n",
    "\n",
    "$$\n",
    "\\langle k(k-1)\\rangle\n",
    "= e^{-\\lambda}\\sum_{k=2}^{\\infty}\\frac{\\lambda^k}{(k-2)!}\n",
    "= \\lambda^2 e^{-\\lambda}\\sum_{k=2}^{\\infty}\\frac{\\lambda^{k-2}}{(k-2)!}.\n",
    "$$\n",
    "\n",
    "Let $j=k-2$:\n",
    "\n",
    "$$\n",
    "\\langle k(k-1)\\rangle\n",
    "= \\lambda^2 e^{-\\lambda}\\sum_{j=0}^{\\infty}\\frac{\\lambda^j}{j!}\n",
    "= \\lambda^2.\n",
    "$$\n",
    "\n",
    "Next, use the identity $k^2 = k(k-1)+k$ to write\n",
    "\n",
    "$$\n",
    "\\langle k^2\\rangle = \\langle k(k-1)\\rangle + \\langle k\\rangle\n",
    "= \\lambda^2 + \\langle k\\rangle.\n",
    "$$\n",
    "\n",
    "Now compute the variance:\n",
    "\n",
    "$$\n",
    "\\mathrm{Var}(k)=\\langle k^2\\rangle-\\langle k\\rangle^2\n",
    "$$\n",
    "\n",
    "$$\n",
    "= (\\lambda^2+\\langle k\\rangle)-\\langle k\\rangle^2.\n",
    "$$\n",
    "\n",
    "From above, $\\langle k\\rangle=\\lambda$, so $\\lambda^2=\\langle k\\rangle^2$. Substituting gives\n",
    "\n",
    "$$\n",
    "\\mathrm{Var}(k)=\\langle k\\rangle^2+\\langle k\\rangle-\\langle k\\rangle^2=\\langle k\\rangle.\n",
    "$$\n",
    "\n",
    "Therefore,\n",
    "\n",
    "$$\n",
    "\\boxed{\\mathrm{Var}(k)=\\langle k\\rangle.}\n",
    "$$\n"
   ]
  },
  {
   "cell_type": "markdown",
   "metadata": {},
   "source": [
    "##### 5. Briefly discuss the physical meaning of this result for counting experiments."
   ]
  },
  {
   "cell_type": "markdown",
   "metadata": {},
   "source": [
    "In a Poisson distribution, the statistical fluctuation is directly determined by the mean number of counts for counting experiments. Because the standard deviation is equal to the square root of the mean ($\\sigma$ = $\\sqrt \\lambda$), higher counts result in higher absolute vairation but lower relative error. Larger total counts will yield more precise measurements. This property specifically applies to events that occur at a constant average rate, such as radioactive decay or particle detections. "
   ]
  },
  {
   "cell_type": "markdown",
   "metadata": {},
   "source": [
    "### Activity 4: Maximum Likelihood Estimation (by hand) for a Gaussian"
   ]
  },
  {
   "cell_type": "markdown",
   "metadata": {},
   "source": [
    "#### Assume a dataset $ \\{x_n\\}_{n=1}^{N} $ is drawn independently from a Gaussian distribution with unknown mean $ \\mu $ and variance $ \\sigma^2 $.\n",
    "\n",
    "##### 1. Write down the likelihood function $ p(\\{x_n\\} \\mid \\mu, \\sigma^2) $.\n"
   ]
  },
  {
   "cell_type": "markdown",
   "metadata": {},
   "source": [
    "Because the observations are independently and identically distributed, the joint probability of the entire data set is the product of the individual Gaussian probabilities\n",
    "**(Bishop Eq. 1.53)**:\n",
    "\n",
    "$$\n",
    "p(\\mathbf{x} \\mid \\mu, \\sigma^2)\n",
    "= \\prod_{n=1}^{N} \\mathcal{N}(x_n \\mid \\mu, \\sigma^2).\n",
    "$$\n",
    "\n",
    "Now the explicit Gaussian density can be substituted for\n",
    "$ \\mathcal{N}(x_n \\mid \\mu, \\sigma^2) $.\n",
    "For the univariate Gaussian, the distribution is given by **Bishop Eq. 2.218**:\n",
    "\n",
    "$$\n",
    "p(x \\mid \\mu, \\sigma^2)\n",
    "= \\frac{1}{(2\\pi\\sigma^2)^{1/2}}\n",
    "\\exp\\!\\left\\{-\\frac{1}{2\\sigma^2}(x-\\mu)^2\\right\\}.\n",
    "$$\n",
    "\n",
    "The resulting likelihood function is therefore\n",
    "\n",
    "$$\n",
    "p(\\mathbf{x} \\mid \\mu, \\sigma^2)\n",
    "= \\prod_{n=1}^{N}\n",
    "\\frac{1}{(2\\pi\\sigma^2)^{1/2}}\n",
    "\\exp\\!\\left\\{-\\frac{(x_n-\\mu)^2}{2\\sigma^2}\\right\\}.\n",
    "$$\n",
    "\n"
   ]
  },
  {
   "cell_type": "markdown",
   "metadata": {},
   "source": [
    "##### 2. Write down the log-likelihood."
   ]
  },
  {
   "cell_type": "markdown",
   "metadata": {},
   "source": [
    "Starting from the likelihood\n",
    "\n",
    "$$\n",
    "p(\\mathbf{x} \\mid \\mu, \\sigma^2)\n",
    "= \\prod_{n=1}^{N}\n",
    "\\frac{1}{(2\\pi\\sigma^2)^{1/2}}\n",
    "\\exp\\!\\left\\{-\\frac{(x_n-\\mu)^2}{2\\sigma^2}\\right\\},\n",
    "$$\n",
    "\n",
    "the log-likelihood is\n",
    "\n",
    "$$\n",
    "\\ln p(\\mathbf{x} \\mid \\mu, \\sigma^2)\n",
    "= \\ln \\prod_{n=1}^{N}\n",
    "\\left[\n",
    "\\frac{1}{(2\\pi\\sigma^2)^{1/2}}\n",
    "\\exp\\!\\left\\{-\\frac{(x_n-\\mu)^2}{2\\sigma^2}\\right\\}\n",
    "\\right].\n",
    "$$\n",
    "\n",
    "Using $\\ln \\prod_n x_n = \\sum_n \\ln x_n$, we obtain\n",
    "\n",
    "$$\n",
    "\\ln p(\\mathbf{x} \\mid \\mu, \\sigma^2)\n",
    "= \\sum_{n=1}^{N}\n",
    "\\ln \\left[\n",
    "\\frac{1}{(2\\pi\\sigma^2)^{1/2}}\n",
    "\\exp\\!\\left\\{-\\frac{(x_n-\\mu)^2}{2\\sigma^2}\\right\\}\n",
    "\\right].\n",
    "$$\n",
    "\n",
    "Using log properties: \n",
    "\n",
    "$$\n",
    "\\ln p(\\mathbf{x} \\mid \\mu, \\sigma^2)\n",
    "= \\sum_{n=1}^{N}\n",
    "\\left[\n",
    "\\ln\\!\\left(\\frac{1}{(2\\pi\\sigma^2)^{1/2}}\\right)\n",
    "+ \\ln\\!\\left(\\exp\\!\\left\\{-\\frac{(x_n-\\mu)^2}{2\\sigma^2}\\right\\}\\right)\n",
    "\\right].\n",
    "$$\n",
    "\n",
    "$$\n",
    "\\ln p(\\mathbf{x} \\mid \\mu, \\sigma^2)\n",
    "= \\sum_{n=1}^{N}\n",
    "\\left[\n",
    "-\\frac{1}{2}\\ln(2\\pi\\sigma^2)\n",
    "-\\frac{(x_n-\\mu)^2}{2\\sigma^2}\n",
    "\\right].\n",
    "$$\n",
    "\n",
    "There is no index in the first term so the log-likelihood simplifies to:\n",
    "\n",
    "$$\n",
    "\\ln p(\\mathbf{x} \\mid \\mu, \\sigma^2)\n",
    "= -\\frac{N}{2}\\ln(2\\pi\\sigma^2)\n",
    "-\\frac{1}{2\\sigma^2}\\sum_{n=1}^{N}(x_n-\\mu)^2.\n",
    "$$\n"
   ]
  },
  {
   "cell_type": "markdown",
   "metadata": {
    "vscode": {
     "languageId": "plaintext"
    }
   },
   "source": [
    "##### 3. Derive the maximum likelihood estimator for $\\mu$."
   ]
  },
  {
   "cell_type": "markdown",
   "metadata": {},
   "source": [
    "Take the derivative of log-likelihood with respect to $\\mu$. Only the second term depends on $\\mu$:\n",
    "\n",
    "$$\n",
    "\\frac{\\partial}{\\partial \\mu}\\ln p(\\mathbf{x} \\mid \\mu, \\sigma^2)\n",
    "$$\n",
    "\n",
    "$$\n",
    "= -\\frac{1}{2\\sigma^2}\\frac{\\partial}{\\partial \\mu}\\sum_{n=1}^{N}(x_n-\\mu)^2.\n",
    "$$\n",
    "\n",
    "Differentiate inside the sum:\n",
    "\n",
    "$$\n",
    "\\frac{\\partial}{\\partial \\mu}(x_n-\\mu)^2 = -2(x_n-\\mu).\n",
    "$$\n",
    "\n",
    "Therefore:\n",
    "\n",
    "$$\n",
    "\\frac{\\partial}{\\partial \\mu}\\ln p(\\mathbf{x} \\mid \\mu, \\sigma^2)\n",
    "= -\\frac{1}{2\\sigma^2}\\sum_{n=1}^{N}\\left[-2(x_n-\\mu)\\right]\n",
    "= \\frac{1}{\\sigma^2}\\sum_{n=1}^{N}(x_n-\\mu).\n",
    "$$\n",
    "\n",
    "Set derivative equal to zero:\n",
    "\n",
    "$$\n",
    "\\frac{1}{\\sigma^2}\\sum_{n=1}^{N}(x_n-\\mu)=0\n",
    "$$\n",
    "$$\n",
    "\\sum_{n=1}^{N}x_n - N\\mu = 0.\n",
    "$$\n",
    "\n",
    "Solve for $ \\mu $:\n",
    "\n",
    "$$\n",
    "\\hat{\\mu} = \\frac{1}{N}\\sum_{n=1}^{N}x_n.\n",
    "$$\n",
    "\n",
    "Thus, the maximum likelihood estimator for the mean is\n",
    "\n",
    "$$\n",
    "\\boxed{\\hat{\\mu} = \\frac{1}{N}\\sum_{n=1}^{N}x_n.}\n",
    "$$\n"
   ]
  },
  {
   "cell_type": "markdown",
   "metadata": {},
   "source": [
    "##### 4. Derive the maximum likelihood estimator for $\\sigma ^2$."
   ]
  },
  {
   "cell_type": "markdown",
   "metadata": {},
   "source": [
    "Starting from the log-likelihood for a Gaussian,\n",
    "\n",
    "$$\n",
    "\\ln p(\\mathbf{x} \\mid \\mu, \\sigma^2)\n",
    "= -\\frac{N}{2}\\ln(2\\pi\\sigma^2)\n",
    "-\\frac{1}{2\\sigma^2}\\sum_{n=1}^{N}(x_n-\\mu)^2,\n",
    "$$\n",
    "\n",
    "Differentiate the log-likelihood with respect to $\\sigma^2$:\n",
    "\n",
    "$$\n",
    "\\frac{\\partial}{\\partial \\sigma^2}\\ln p(\\mathbf{x} \\mid \\mu, \\sigma^2)\n",
    "= -\\frac{N}{2}\\frac{1}{\\sigma^2}\n",
    "+ \\frac{1}{2(\\sigma^2)^2}\\sum_{n=1}^{N}(x_n-\\mu)^2.\n",
    "$$\n",
    "\n",
    "Set the derivative equal to zero:\n",
    "\n",
    "$$\n",
    "-\\frac{N}{2}\\frac{1}{\\sigma^2}\n",
    "+ \\frac{1}{2(\\sigma^2)^2}\\sum_{n=1}^{N}(x_n-\\mu)^2 = 0.\n",
    "$$\n",
    "\n",
    "$$\n",
    "- N\\sigma^2 + \\sum_{n=1}^{N}(x_n-\\mu)^2 = 0.\n",
    "$$\n",
    "\n",
    "$$\n",
    "\\hat{\\sigma}^2\n",
    "= \\frac{1}{N}\\sum_{n=1}^{N}(x_n-\\mu)^2.\n",
    "$$\n",
    "\n",
    "Replacing $ \\mu $ with its maximum likelihood estimate:\n",
    "$$\n",
    "\\boxed{\n",
    "\\hat{\\sigma}^2\n",
    "= \\frac{1}{N}\\sum_{n=1}^{N}\\bigl(x_n-\\hat{\\mu}\\bigr)^2\n",
    "}.\n",
    "$$\n"
   ]
  },
  {
   "cell_type": "markdown",
   "metadata": {},
   "source": [
    "##### 5. Compare your expression for $\\sigma ^2$ with the unbiased sample variance estimator. Briefly explain the difference, and discuss when this difference is relevant. "
   ]
  },
  {
   "cell_type": "markdown",
   "metadata": {},
   "source": [
    "The maximum likelihood estimator for the variance is\n",
    "\n",
    "$$\n",
    "\\hat{\\sigma}^2 = \\frac{1}{N}\\sum_{n=1}^{N}(x_n-\\hat{\\mu})^2,\n",
    "$$\n",
    "\n",
    "where $ \\hat{\\mu} = \\frac{1}{N}\\sum_{n=1}^{N}x_n $.\n",
    "The unbiased sample variance estimator is given by **Bishop Eq. 1.59**:\n",
    "\n",
    "$$\n",
    "\\sigma^2 = \\frac{1}{N-1}\\sum_{n=1}^{N}(x_n-\\mu)^2.\n",
    "$$\n",
    "\n",
    "The difference between these two estimators is the factor of $N-1$ in the denominator of the unbiased estimate.\n",
    "The maximum likelihood estimator divides by $ N $, which results in a slight\n",
    "downward bias because the same data are used to estimate both the mean and the\n",
    "variance.\n",
    "The unbiased estimator divides by $ N-1 $, correcting for the loss of one\n",
    "degree of freedom associated with estimating the mean. This also removes the bias of maximum liklihood.\n"
   ]
  },
  {
   "cell_type": "markdown",
   "metadata": {},
   "source": []
  },
  {
   "cell_type": "markdown",
   "metadata": {},
   "source": []
  }
 ],
 "metadata": {
  "language_info": {
   "name": "python"
  }
 },
 "nbformat": 4,
 "nbformat_minor": 2
}
