{
 "cells": [
  {
   "cell_type": "markdown",
   "metadata": {},
   "source": [
    "### Activity 2: Poisson distribution - mean and variance"
   ]
  },
  {
   "cell_type": "markdown",
   "metadata": {},
   "source": [
    "#### Consider a Poisson process with a rate parameter $\\lambda$. The probability of observing k events in a fixed interval is given by the Poisson distribution. \n",
    "\n",
    "##### 1. Write down the Poisson probability mass function $p(k \\mid \\lambda)$."
   ]
  },
  {
   "cell_type": "markdown",
   "metadata": {},
   "source": [
    "The probability mass function for observing \\( k \\) events in a fixed interval is\n",
    "\n",
    "$$\n",
    "p(k \\mid \\lambda) = \\frac{\\lambda^k e^{-\\lambda}}{k!},\n",
    "$$\n",
    "\n",
    "where \\( k = 0, 1, 2,... \\).\n"
   ]
  },
  {
   "cell_type": "markdown",
   "metadata": {},
   "source": [
    "##### 2. Compute the expectation value $<k>$."
   ]
  },
  {
   "cell_type": "markdown",
   "metadata": {},
   "source": [
    "The expectation value of \\( k \\) for a Poisson distribution is defined as\n",
    "\n",
    "$$\n",
    "\\langle k \\rangle = \\sum_{k=0}^{\\infty} k \\, p(k \\mid \\lambda).\n",
    "$$\n",
    "\n",
    "Plugging in the probability mass function \\( p(k \\mid \\lambda) \\):\n",
    "\n",
    "$$\n",
    "\\langle k \\rangle\n",
    "= \\sum_{k=0}^{\\infty} k \\frac{\\lambda^k e^{-\\lambda}}{k!}.\n",
    "$$\n",
    "\n",
    "The \\( k = 0 \\) term vanishes, so we may write\n",
    "\n",
    "$$\n",
    "\\langle k \\rangle\n",
    "= \\sum_{k=1}^{\\infty} k \\frac{\\lambda^k e^{-\\lambda}}{k!}.\n",
    "$$\n",
    "\n",
    "Using the identity\n",
    "\n",
    "$$\n",
    "\\frac{k}{k!} = \\frac{1}{(k-1)!},\n",
    "$$\n",
    "\n",
    "we obtain\n",
    "\n",
    "$$\n",
    "\\langle k \\rangle\n",
    "= e^{-\\lambda} \\sum_{k=1}^{\\infty} \\frac{\\lambda^k}{(k-1)!}.\n",
    "$$\n",
    "\n",
    "Factoring out a power of \\( \\lambda \\),\n",
    "\n",
    "$$\n",
    "\\langle k \\rangle\n",
    "= \\lambda e^{-\\lambda} \\sum_{k=1}^{\\infty} \\frac{\\lambda^{k-1}}{(k-1)!}.\n",
    "$$\n",
    "\n",
    "Letting \\( j = k - 1 \\), this becomes\n",
    "\n",
    "$$\n",
    "\\langle k \\rangle\n",
    "= \\lambda e^{-\\lambda} \\sum_{j=0}^{\\infty} \\frac{\\lambda^j}{j!}.\n",
    "$$\n",
    "\n",
    "Using the Taylor series expansion of the exponential function,\n",
    "\n",
    "$$\n",
    "\\sum_{j=0}^{\\infty} \\frac{\\lambda^j}{j!} = e^{\\lambda},\n",
    "$$\n",
    "\n",
    "we find\n",
    "\n",
    "$$\n",
    "\\langle k \\rangle = \\lambda e^{-\\lambda} e^{\\lambda} = \\lambda.\n",
    "$$\n",
    "\n",
    "Therefore,\n",
    "\n",
    "$$\n",
    "\\boxed{\\langle k \\rangle = \\lambda.}\n",
    "$$\n"
   ]
  },
  {
   "cell_type": "markdown",
   "metadata": {},
   "source": [
    "##### 3. Compute the variance $\\mathrm{Var}(k)$."
   ]
  },
  {
   "cell_type": "markdown",
   "metadata": {},
   "source": [
    "We begin with the definition of the variance,\n",
    "\n",
    "$$\n",
    "\\mathrm{Var}(k) = \\langle k^2 \\rangle - \\langle k \\rangle^2.\n",
    "$$\n",
    "\n",
    "For a Poisson distribution with parameter \\( \\lambda \\), the expectation value is\n",
    "\n",
    "$$\n",
    "\\langle k \\rangle = \\lambda.\n",
    "$$\n",
    "\n",
    "We now compute \\( \\langle k^2 \\rangle \\):\n",
    "\n",
    "$$\n",
    "\\langle k^2 \\rangle\n",
    "= \\sum_{k=0}^{\\infty} k^2 \\, p(k \\mid \\lambda)\n",
    "= \\sum_{k=0}^{\\infty} k^2 \\frac{\\lambda^k e^{-\\lambda}}{k!}.\n",
    "$$\n",
    "\n",
    "Rewrite \\( k^2 \\) as\n",
    "\n",
    "$$\n",
    "k^2 = k(k-1) + k.\n",
    "$$\n",
    "\n",
    "Then\n",
    "\n",
    "$$\n",
    "\\langle k^2 \\rangle\n",
    "= \\sum_{k=0}^{\\infty} k(k-1)\\frac{\\lambda^k e^{-\\lambda}}{k!}\n",
    "+ \\sum_{k=0}^{\\infty} k\\frac{\\lambda^k e^{-\\lambda}}{k!}.\n",
    "$$\n",
    "\n",
    "The second sum is simply\n",
    "\n",
    "$$\n",
    "\\langle k \\rangle = \\lambda.\n",
    "$$\n",
    "\n",
    "For the first sum, note that\n",
    "\n",
    "$$\n",
    "\\frac{k(k-1)}{k!} = \\frac{1}{(k-2)!},\n",
    "$$\n",
    "\n",
    "and the terms with \\( k=0,1 \\) vanish. Thus,\n",
    "\n",
    "$$\n",
    "\\sum_{k=0}^{\\infty} k(k-1)\\frac{\\lambda^k e^{-\\lambda}}{k!}\n",
    "= e^{-\\lambda} \\sum_{k=2}^{\\infty} \\frac{\\lambda^k}{(k-2)!}.\n",
    "$$\n",
    "\n",
    "Factor out \\( \\lambda^2 \\):\n",
    "\n",
    "$$\n",
    "= \\lambda^2 e^{-\\lambda} \\sum_{k=2}^{\\infty} \\frac{\\lambda^{k-2}}{(k-2)!}.\n",
    "$$\n",
    "\n",
    "Letting \\( j = k - 2 \\),\n",
    "\n",
    "$$\n",
    "= \\lambda^2 e^{-\\lambda} \\sum_{j=0}^{\\infty} \\frac{\\lambda^j}{j!}\n",
    "= \\lambda^2.\n",
    "$$\n",
    "\n",
    "Therefore,\n",
    "\n",
    "$$\n",
    "\\langle k^2 \\rangle = \\lambda^2 + \\lambda.\n",
    "$$\n",
    "\n",
    "Substituting into the variance,\n",
    "\n",
    "$$\n",
    "\\mathrm{Var}(k)\n",
    "= \\langle k^2 \\rangle - \\langle k \\rangle^2\n",
    "= (\\lambda^2 + \\lambda) - \\lambda^2\n",
    "= \\lambda.\n",
    "$$\n",
    "\n",
    "Hence,\n",
    "\n",
    "$$\n",
    "\\boxed{\\mathrm{Var}(k) = \\langle k \\rangle.}\n",
    "$$\n"
   ]
  },
  {
   "cell_type": "markdown",
   "metadata": {},
   "source": [
    "##### 4. Show explicitly that $\\mathrm{Var}(k)$."
   ]
  },
  {
   "cell_type": "markdown",
   "metadata": {},
   "source": [
    "Start with the Poisson pmf\n",
    "\n",
    "$$\n",
    "p(k\\mid \\lambda)=\\frac{\\lambda^k e^{-\\lambda}}{k!}, \\qquad k=0,1,2,\\dots\n",
    "$$\n",
    "\n",
    "The expectation value is\n",
    "\n",
    "$$\n",
    "\\langle k\\rangle=\\sum_{k=0}^{\\infty} k\\,p(k\\mid\\lambda)\n",
    "= e^{-\\lambda}\\sum_{k=1}^{\\infty} k\\frac{\\lambda^k}{k!}\n",
    "= e^{-\\lambda}\\sum_{k=1}^{\\infty}\\frac{\\lambda^k}{(k-1)!}.\n",
    "$$\n",
    "\n",
    "Factor out one power of $\\lambda$ and shift the index \\(j=k-1\\):\n",
    "\n",
    "$$\n",
    "\\langle k\\rangle\n",
    "= \\lambda e^{-\\lambda}\\sum_{k=1}^{\\infty}\\frac{\\lambda^{k-1}}{(k-1)!}\n",
    "= \\lambda e^{-\\lambda}\\sum_{j=0}^{\\infty}\\frac{\\lambda^j}{j!}\n",
    "= \\lambda.\n",
    "$$\n",
    "\n",
    "Now compute $\\langle k(k-1)\\rangle$:\n",
    "\n",
    "$$\n",
    "\\langle k(k-1)\\rangle\n",
    "= \\sum_{k=0}^{\\infty} k(k-1)p(k\\mid\\lambda)\n",
    "= e^{-\\lambda}\\sum_{k=2}^{\\infty} k(k-1)\\frac{\\lambda^k}{k!}.\n",
    "$$\n",
    "\n",
    "Use the identity\n",
    "\n",
    "$$\n",
    "\\frac{k(k-1)}{k!}=\\frac{1}{(k-2)!},\n",
    "$$\n",
    "\n",
    "so\n",
    "\n",
    "$$\n",
    "\\langle k(k-1)\\rangle\n",
    "= e^{-\\lambda}\\sum_{k=2}^{\\infty}\\frac{\\lambda^k}{(k-2)!}\n",
    "= \\lambda^2 e^{-\\lambda}\\sum_{k=2}^{\\infty}\\frac{\\lambda^{k-2}}{(k-2)!}.\n",
    "$$\n",
    "\n",
    "Let \\(j=k-2\\):\n",
    "\n",
    "$$\n",
    "\\langle k(k-1)\\rangle\n",
    "= \\lambda^2 e^{-\\lambda}\\sum_{j=0}^{\\infty}\\frac{\\lambda^j}{j!}\n",
    "= \\lambda^2.\n",
    "$$\n",
    "\n",
    "Next, use \\(k^2 = k(k-1)+k\\) to write\n",
    "\n",
    "$$\n",
    "\\langle k^2\\rangle = \\langle k(k-1)\\rangle + \\langle k\\rangle\n",
    "= \\lambda^2 + \\langle k\\rangle.\n",
    "$$\n",
    "\n",
    "Now compute the variance:\n",
    "\n",
    "$$\n",
    "\\mathrm{Var}(k)=\\langle k^2\\rangle-\\langle k\\rangle^2\n",
    "= (\\lambda^2+\\langle k\\rangle)-\\langle k\\rangle^2.\n",
    "$$\n",
    "\n",
    "But from above, $\\langle k\\rangle=\\lambda$, so $\\lambda^2=\\langle k\\rangle^2$. Substituting gives\n",
    "\n",
    "$$\n",
    "\\mathrm{Var}(k)=\\langle k\\rangle^2+\\langle k\\rangle-\\langle k\\rangle^2=\\langle k\\rangle.\n",
    "$$\n",
    "\n",
    "Therefore,\n",
    "\n",
    "$$\n",
    "\\boxed{\\mathrm{Var}(k)=\\langle k\\rangle.}\n",
    "$$\n"
   ]
  },
  {
   "cell_type": "markdown",
   "metadata": {},
   "source": [
    "##### 5. Briefly discuss the physical meaning of this result for counting experiments."
   ]
  },
  {
   "cell_type": "markdown",
   "metadata": {},
   "source": [
    "In a Poisson distribution, the statistical fluctuation is directly determines by the mean number of counts"
   ]
  }
 ],
 "metadata": {
  "language_info": {
   "name": "python"
  }
 },
 "nbformat": 4,
 "nbformat_minor": 2
}
